\documentclass[]{article}


%导入宏包
\usepackage{ctex}
\usepackage{graphics}
\usepackage{amsmath,amssymb}
\usepackage{amsthm}
\usepackage{pst-blur}
\usepackage{pstricks-add}
\usepackage{pstricks}
\usepackage{pstricks-pdf}
\usepackage{pgf,tikz,pgfplots}
\usepackage{mathrsfs}
\usepackage{xcolor}
\usepackage{eso-pic}
%\usepackage{background}
\usepackage{xeCJK}
    \xeCJKsetup{CJKmath=true}
%\usepackage{wallpaper}


%opening
\title{}
\author{}
\date{}
\setlength\parindent{0em}

\begin{document}
%\maketitle
\section{安振平5461}{
已知,$a,b,c>0,(a+b)(b+c)(c+a)=1$,求证:$ab+bc+ca+2abc \leq 1\leq a^2+b^2+c^2+2abc$.

\begin{proof}
条件$\Longleftrightarrow \sum\limits_{sym}a^2b+2abc=1$
\begin{enumerate}
    \item 左边
    \begin{equation}\nonumber
        \Longleftrightarrow \sum_{sym}a^2b \geq ab+bc+ac
    \end{equation}
    由均值不等式
    \begin{equation}\nonumber
    \begin{split}\nonumber
        a^2b+b^2a\geq 2\sqrt{a^3b^3}\\
        b^2c+c^2b\geq 2\sqrt{b^3c^3}\\
        c^2a+a^2c\geq 2\sqrt{c^3a^3}
    \end{split}
    \end{equation}
    由均值不等式
    \begin{equation}\nonumber
        ab+bc+ca+2abc=1\leq ab+bc+ca+2\frac{(ab+bc+ca)^{\frac{3}{2}}}{3}
    \end{equation}
    解得$ab+bc+ca\geq \frac{3}{2}$.
    由幂平均不等式
    \begin{equation}\nonumber
        2\sqrt{a^3b^3}+2\sqrt{b^3c^3}+2\sqrt{c^3a^3}\geq 6(\frac{(ab+bc+ca)}{3})^{\frac{3}{2}}\geq ab+bc+ca
    \end{equation}
    \item 右边
    \begin{equation}\nonumber
        \Longleftrightarrow a^2+b^2+c^2\geq \sum_{sym}a^2b
    \end{equation}
    而
    \begin{equation}\nonumber
        a^2+b^2+c^2=\frac{\sum a^3+\sum\limits_{sym}a^2b}{\sum a}
    \end{equation}
    待证式
    \begin{equation}\nonumber
        \Longleftrightarrow (\sum\limits_{sym}a^2b+2abc)(\frac{\sum a^3+\sum\limits_{sym}a^2b}{\sum a})^3-(\sum\limits_{sym}a^2b)^3\geq 0 
    \end{equation}
    展开
    \begin{equation}\nonumber
    \begin{split}
        \Longleftrightarrow (\sum a^3)^3(\sum_{sym}a^2b)+2abc(\sum a^3)^3+3(\sum a^3)^2(\sum_{sym}a^2b)^2+\\6abc(\sum a^3)(\sum_{sym}a^2b)+2(\sum a^3)(\sum_{sym}a^2b)^3+6abc(\sum a^3)(\sum_{sym}a^2b)^2\\-2(\sum_{sym}a^2b)^4-4abc(\sum_{sym}a^2b)^3\geq 0
    \end{split}
    \end{equation}
    由舒尔不等式知
    \begin{equation}\nonumber
        \sum a^3+3abc\geq \sum\limits_{sym}a^2b
    \end{equation}
     \begin{equation}\nonumber
    \begin{split}
        \Longleftrightarrow (\sum a^3)^3(\sum_{sym}a^2b)+2abc(\sum a^3)^3+3(\sum a^3)^2(\sum_{sym}a^2b)^2+\\6abc(\sum a^3)(\sum_{sym}a^2b)+6abc(\sum a^3)(\sum_{sym}a^2b)^2\\-10abc(\sum_{sym}a^2b)^3+2(\sum_{sym}a^2b)^3(\sum a^3-\sum_{sym}a^2b+3abc)\geq 0
    \end{split}
    \end{equation}   
    \begin{equation}\nonumber
    \begin{split}
         \Longleftrightarrow (\sum a^3)^3(\sum_{sym}a^2b)+2abc(\sum a^3)^3+3(\sum a^3)^2(\sum_{sym}a^2b)^2+\\6abc(\sum a^3)(\sum_{sym}a^2b)+6abc(\sum a^3)(\sum_{sym}a^2b)^2-10abc(\sum_{sym}a^2b)^3\geq 0
    \end{split}
    \end{equation}
    由均值不等式知
    \begin{equation}\nonumber
        \sum a^3\geq 3abc
    \end{equation}
    \begin{equation}\nonumber
        \sum a^3 \geq \frac{1}{2}\sum_{sym}a^2b
    \end{equation}
    \begin{equation}\nonumber
        (\sum a^3)^3(\sum_{sym}a^2b)\geq \frac{3}{4}abc(\sum_{sym}a^2b)^3
    \end{equation}
    \begin{equation}\nonumber
        2abc(\sum a^3)^3\geq \frac{1}{4}abc(\sum_{sym}a^2b)^3
    \end{equation}
    \begin{equation}\nonumber
        3(\sum a^3)^2(\sum_{sym}a^2b)\geq \frac{9}{2}abc(\sum_{sym}a^2b)^3
    \end{equation}
    \begin{equation}\nonumber
        6abc(\sum a^3)^2(\sum_{sym}a^2b)\geq \frac{3}{2}abc(\sum_{sym}a^2b)^3
    \end{equation}
    \begin{equation}\nonumber
        6abc(\sum a^3)(\sum_{sym}a^2b)^2\geq 3abc(\sum_{sym}a^2b)^3
    \end{equation}
    \begin{equation}\nonumber
        \begin{split}
            \Longrightarrow (\sum a^3)^3(\sum_{sym}a^2b)+2abc(\sum a^3)^3+3(\sum a^3)^2(\sum_{sym}a^2b)^2+\\6abc(\sum a^3)(\sum_{sym}a^2b)+6abc(\sum a^3)(\sum_{sym}a^2b)^2-10abc(\sum_{sym}a^2b)^3\geq 0
        \end{split}
    \end{equation}
    成立.
\end{enumerate}
\end{proof}
}
\end{document}